Convert DB to use nown.

nown.v
@@ -65,10 +65,14 @@ rewrite nown_token_difference //.
 by iDestruct "t" as "[t _]".
 Qed.
 
-Definition nown `{!inG Σ A} γ N (a : A) : iProp :=
+Section NOwnLaws.
+
+Context `{!inG Σ A}.
+
+Definition nown γ N (a : A) : iProp :=
   ∃ γ', nown_ptr γ N γ' ∧ own γ' a.
 
-Lemma nown_alloc `{!inG Σ A} γ N E (a : A) :
+Lemma nown_alloc γ N E (a : A) :
   ↑N ⊆ E → ✓ a → nown_token γ E ==∗ nown γ N a ∗ nown_token γ (E ∖ ↑N).
 Proof.
 intros sub valid_a. iIntros "token".
@@ -78,12 +82,12 @@ iDestruct "token" as "[tok1 tok2]". iFrame. iExists γ'. iFrame.
 by iApply (gmeta_set with "tok1").
 Qed.
 
-Lemma nown_valid `{!inG Σ A} γ N (a : A) : nown γ N a -∗ ✓ a.
+Lemma nown_valid γ N (a : A) : nown γ N a -∗ ✓ a.
 Proof.
 iIntros "(%γ' & #own_γ & own)". iApply (own_valid with "own").
 Qed.
 
-Lemma nown_valid_2 `{!inG Σ A} γ N (a1 a2 : A) :
+Lemma nown_valid_2 γ N (a1 a2 : A) :
   nown γ N a1 -∗ nown γ N a2 -∗ ✓ (a1 ⋅ a2).
 Proof.
 iIntros "(%γ1 & #own_γ1 & own1) (%γ2 & #own_γ2 & own2)".
@@ -91,7 +95,7 @@ iPoseProof (nown_ptr_agree with "own_γ1 own_γ2") as "<-".
 by iApply (own_valid_2 with "own1 own2").
 Qed.
 
-Lemma nown_update `{!inG Σ A} γ N (a a' : A) :
+Lemma nown_update γ N (a a' : A) :
   a ~~> a' → nown γ N a ==∗ nown γ N a'.
 Proof.
 iIntros (?) "(%γ' & #? & own)".
@@ -100,16 +104,24 @@ iModIntro. iExists γ'. eauto.
 Qed.
 
 #[global]
-Instance nown_core_persistent `{!inG Σ A} γ N (a : A) :
+Instance nown_core_persistent γ N (a : A) :
   CoreId a → Persistent (nown γ N a).
 Proof. apply _. Qed.
 
 #[global]
-Instance nown_timeless `{!inG Σ A} γ N (a : A) :
+Instance nown_timeless γ N (a : A) :
   Discrete a → Timeless (nown γ N a).
 Proof. apply _. Qed.
 
-Lemma nown_op `{!inG Σ A} γ N (a1 a2 : A) :
+#[global]
+Instance nown_ne γ N : NonExpansive (nown γ N).
+Proof. solve_proper. Qed.
+
+#[global]
+Instance nown_proper γ N : Proper ((≡) ==> (≡)) (nown γ N).
+Proof. solve_proper. Qed.
+
+Lemma nown_op γ N (a1 a2 : A) :
   nown γ N (a1 ⋅ a2) ⊣⊢ nown γ N a1 ∗ nown γ N a2.
 Proof.
 iSplit.
@@ -120,7 +132,42 @@ iSplit.
   iExists γ1. iSplit => //. by iSplitL "own1".
 Qed.
 
+#[global]
+Instance from_sep_nown γ N (a b1 b2 : A) :
+  IsOp a b1 b2 → FromSep (nown γ N a) (nown γ N b1) (nown γ N b2).
+Proof.
+by rewrite /IsOp /FromSep => ->; rewrite nown_op.
+Qed.
+
+#[global]
+Instance into_sep_nown γ N (a b1 b2 : A) :
+  IsOp a b1 b2 → IntoSep (nown γ N a) (nown γ N b1) (nown γ N b2).
+Proof.
+by rewrite /IsOp /IntoSep => ->; rewrite nown_op.
+Qed.
+
+Lemma nown_mono γ N (a1 a2 : A) : a1 ≼ a2 → nown γ N a2 -∗ nown γ N a1.
+Proof.
+case => ? ->.
+rewrite nown_op.
+by iIntros "[??]".
+Qed.
+
+Lemma nown_update_2 γ N (a1 a2 a' : A) :
+  a1 ⋅ a2 ~~> a' →
+  nown γ N a1 -∗
+  nown γ N a2 ==∗
+  nown γ N a'.
+Proof.
+iIntros "% H1 H2".
+iMod (nown_update with "[H1 H2]") as "H" => //.
+by iSplitL "H1".
+Qed.
+
+End NOwnLaws.
+
 End NOwn.
 
+#[global] Typeclasses Opaque nown nown_token.
 Arguments nown_alloc {Σ _ A _ γ} N {_} a.
 Arguments nown_token_difference {Σ _} E1 E2 γ.
